theories/ConfigUtils.v
@@ -11,6 +11,7 @@ From Peregrine Require Import RustBackend.
 From Peregrine Require Import ElmBackend.
 From Peregrine Require Import OCamlBackend.
 From Peregrine Require Import CakeMLBackend.
+From Peregrine Require Import FSharpBackend.
 From Peregrine Require Import CBackend.
 From Peregrine Require Import WasmBackend.
 From Peregrine Require Import EvalBackend.
@@ -174,6 +175,21 @@ Section BackendConfigOptional.
 
   Definition mk_cakeml_config (o : cakeml_config') : cakeml_config := tt.
 
+  (* F# *)
+  Record fsharp_config' := {
+    fsharp_namespace'        : option string;
+    fsharp_print_full_names' : option bool;
+  }.
+  Definition empty_fsharp_config' : fsharp_config' := {|
+    fsharp_namespace'        := None;
+    fsharp_print_full_names' := None;
+  |}.
+
+  Definition mk_fsharp_config (o : fsharp_config') : fsharp_config := {|
+    fsharp_namespace        := get_optional o default_fsharp_config fsharp_namespace' fsharp_namespace;
+    fsharp_print_full_names := get_optional o default_fsharp_config fsharp_print_full_names' fsharp_print_full_names;
+  |}.
+
   Record eval_config' := {
     copts'    : option certirocq_config';
     fuel'     : nat;
@@ -227,6 +243,7 @@ Section BackendConfigOptional.
   | Wasm'   : wasm_config' -> backend_config'
   | OCaml'  : ocaml_config' -> backend_config'
   | CakeML' : cakeml_config' -> backend_config'
+  | FSharp' : fsharp_config' -> backend_config'
   | Eval'   : eval_config' -> backend_config'
   | AST'    : ast_config' -> backend_config'.
   Definition mk_backend_config (o : backend_config') : backend_config :=
@@ -237,6 +254,7 @@ Section BackendConfigOptional.
     | Wasm' o   => Wasm (mk_certirocq_config default_wasm_config o)
     | OCaml' o  => OCaml (mk_ocaml_config o)
     | CakeML' o => CakeML (mk_cakeml_config o)
+    | FSharp' o => FSharp (mk_fsharp_config o)
     | Eval' o   => Eval (mk_eval_config o)
     | AST' o    => AST (mk_ast_config o)
     end.
@@ -313,6 +331,7 @@ Section GeneralConfigOptional.
       | Wasm' _   => get_default_phases_opt wasm_phases
       | OCaml' _  => get_default_phases_opt ocaml_phases
       | CakeML' _ => get_default_phases_opt cakeml_phases
+      | FSharp' _ => get_default_phases_opt fsharp_phases
       | Eval' _   => get_default_phases_opt eval_phases
       | AST' _   => get_default_phases_opt ast_phases
       end in
@@ -325,6 +344,7 @@ Section GeneralConfigOptional.
       | Wasm' _   => enforce_phases o def_opt wasm_phases
       | OCaml' _  => enforce_phases o def_opt ocaml_phases
       | CakeML' _ => enforce_phases o def_opt cakeml_phases
+      | FSharp' _ => enforce_phases o def_opt fsharp_phases
       | Eval' _   => enforce_phases o def_opt eval_phases
       | AST' _   => enforce_phases o def_opt ast_phases
       end
@@ -407,6 +427,12 @@ Section GeneralConfigOptional.
   Definition is_cakeml_config (o : config) : bool :=
     match o.(backend_opts) with
     | CakeML _ => true
+    | _ => false
+    end.
+
+  Definition is_fsharp_config (o : config) : bool :=
+    match o.(backend_opts) with
+    | FSharp _ => true
     | _ => false
     end.
 
